TM/Basic/WriteString.v
@@ -1,53 +1,113 @@
-Require Import Basic.Mono Basic  Compound Combinators.SequentialComposition.
+Require Import TM.TM TM.Basic.Mono TM.Combinators.SequentialComposition.
 
-Section write_string.
+(*
+Fixpoint stroverwrite (sig : Type) (str1 str2 : list sig) : list sig :=
+  match str1, str2 with
+  | str1, nil => str1
+  | nil, str2 => str2
+  | s1::str1', s2::str2' => s2 :: stroverwrite str1' str2'
+  end.
+
+  Lemma stroverwrite_nil (str1 : list sig) :
+    stroverwrite str1 [] = str1.
+  Proof. destruct str1; cbn; reflexivity. Qed.
+*)
+
+Section Write_String.
 
   Variable sig : finType.
-  Variable tapes_no : nat.
-
-  Variable on_tape : nat.
-  Hypothesis is_a_tape : on_tape < S tapes_no.
-
-  Fixpoint Write_string (l : list sig) : {M :  mTM sig tapes_no & states M -> unit} :=
+  
+  Fixpoint Write_String (l : list sig) : {M : mTM sig 0 & states M -> unit} :=
     match l with
-    | [] => Nop tapes_no sig tt
-    | e :: l0 => Write is_a_tape e;; Move _ is_a_tape R;; Write_string l0
+    | [] => mono_Nop sig tt
+    | e :: l0 => Write e ;; Move _ R ;; Write_String l0
     end.
 
-  Definition Write_string_R l :=
-    fun (t t' : tape sig) => exists R,
-        t' = mk_rtape (rev l ++ left t) R.
+  (*
+  Fixpoint Tape_Write_String (t : tape sig) (str : list sig) :=
+    match t, str with
+    | t, nil => t
+    | niltape _, s :: str' => Tape_Write_String (rightof s []) str'
+    | leftof l rs, s :: str' => Tape_Write_String (midtape [s] l rs) str'
+    | midtape ls m nil, s :: str' => Tape_Write_String (rightof s ls) str'
+    | midtape ls m (r :: rs), s :: str' => Tape_Write_String (midtape (s :: ls) r rs) str'
+    | rightof r ls, s :: str' => Tape_Write_String (rightof s (r :: ls)) str'
+    end.
+   *)
+
+  Fixpoint Tape_Write_String (t : tape sig) (str : list sig) :=
+    match str with
+    | nil => t
+    | s :: str' => Tape_Write_String (tape_move_mono t (Some s, R)) str'
+    end.
   
-  Lemma Write_string_sem x l :
-    Write_string (x :: l) ⊨(4 + 4 * |l|) ⇑[is_a_tape] ignoreParam (Write_string_R (x :: l)).
+  
+  Lemma Tape_Write_String_nil (t : tape sig) :
+    Tape_Write_String t nil = t.
+  Proof. destruct t; cbn; auto. Qed.
+
+(*
+End write_string.
+Section Test.
+  Inductive Digit := zero | one | two | three | four | five | six | seven | eight | nine.
+  Instance digit_eq : eq_dec Digit.
+  Proof. unfold dec. intros x y. decide equality. Defined.
+  Instance digit_fin : finTypeC (EqType Digit).
   Proof.
-    revert x. induction l; intros.
-    - unfold Write_string.
-      TMstep. eapply Seq_total. eapply write_sem. eapply Seq_total.
-      eapply move_sem. eapply Nop_total. omega.
-      autorewrite lift.
-      repeat setoid_rewrite lift_hideParam.
-      rewrite ignore_hideParam; try now econstructor. TMcorrect.
-      intros ? ([] & ?) ?. TMnormalise. subst. cbn in *.
-      destruct x2; TMnormalise. unfold MoveR, Write_string_R in *.
-      cbn in *. destruct b; TMnormalise; subst.
-      + inv H0. destruct _. exists nil; eauto. now exists (e :: l).
-      + inv H.
-    - unfold Write_string. TMstep.
-      eapply Seq_total. eapply write_sem.
-      eapply Seq_total. eapply move_sem.
-      eapply IHl. cbn. omega.
-      autorewrite lift.
-      repeat setoid_rewrite lift_hideParam.
-      rewrite ignore_hideParam; try now econstructor. TMcorrect.
-      intros ? ([] & ?) ?.
-      repeat TMnormaliseH1. subst. cbn in x2; destruct x2.
-      unfold MoveR in H0. unfold Write_string_R in H1.
-      unfold Write_string_R. cbn -[Write_string] in *.
-      destruct b; subst.
-      + destruct H0. destruct H0. destruct H1. subst. inv H0.
-        destruct _; cbn; exists x2; now autorewrite with list.
-      + exfalso. clear IHl. TMnormalise. inv H.
+    apply FinTypeC with (enum := [zero; one; two; three; four; five; six; seven; eight; nine]).
+    intros. destruct x; cbn; reflexivity.
+  Defined.
+  Compute Tape_Write_String (rightof three [two; one]) [].
+  Compute Tape_Write_String (rightof two [one]) [three].
+  Compute Tape_Write_String (rightof one []) [two; three].
+  Compute Tape_Write_String (niltape _) [zero; one; two].
+  Compute Tape_Write_String (niltape _) [zero; one].
+  Compute Tape_Write_String (niltape _) [zero].
+  Compute Tape_Write_String (midtape [zero;one] two [three;four;five]) [].
+  Compute Tape_Write_String (midtape [zero;one] two [three;four;five]) [six].
+  Compute Tape_Write_String (midtape [zero;one] two [three;four;five]) [six;seven].
+  Compute Tape_Write_String (midtape [zero;one] two [three;four;five]) [six;seven;eight].
+  Compute Tape_Write_String (midtape [zero;one] two [three;four;five]) [six;seven;eight;nine].
+End Test.
+*)
+
+  Fixpoint Write_string_sem_fix (str : list sig) : Rel (tapes sig 1) (unit * tapes sig 1) :=
+    match str with
+    | nil => mono_Nop_R tt
+    | s :: str' => Write_R s ∘ hideParam (Move_R R ∘ hideParam (Write_string_sem_fix str'))
+    end.
+    
+  Lemma Write_string_fix_Sem (str : list sig) :
+    Write_String str ⊨(4 * |str|) (Write_string_sem_fix str).
+  Proof.
+    induction str.
+    - cbn. apply mono_Nop_Sem.
+    - cbn.
+      replace (S ((| str |) + S ((| str |) + S ((| str |) + S ((| str |) + 0)))))
+        with (1 + 1 + (1 + 1 + (4 * (|str|)))); [ | cbn; omega].
+      apply Seq_total.
+      + apply Write_Sem.
+      + apply Seq_total.
+        * apply Move_Sem.
+        * apply IHstr.
+  Qed.
+  
+  Definition Write_String_R str :=
+    Mono.Mk_R_p (F := FinType (EqType unit))
+                (ignoreParam (fun (t t' : tape sig) => t' = Tape_Write_String t str)).
+
+  Lemma Write_string_Sem str :
+    Write_String str ⊨(4 * |str|) (Write_String_R str).
+  Proof.
+    eapply RealiseIn_monotone with (k1 := 4 * (|str|)); [now apply Write_string_fix_Sem | omega | ]. 
+    induction str.
+    - hnf. intros x ([], y) (H1 & H2). hnf in *. subst. now rewrite Tape_Write_String_nil.
+    - intros t1 ([], t2) (([]&t3)&H1&((b&t4)&H2&H3)). hnf in H1, H2, H3. destruct_tapes. cbn in H1, H2, H3. cbn. subst.
+      specialize (IHstr _ _ H3). clear H3. cbn in IHstr. hnf in IHstr. hnf. subst.
+      destruct b.
+      + destruct H2 as (H2&(c&H2')). cbn in H2, H2'. injection H2'. intros ->. clear H2'. subst.
+        destruct h eqn:E1, str eqn:E2; cbn; auto.
+      + destruct H2 as (H2&_). cbn in H2. congruence.
   Qed.
 
-End write_string.
+End Write_String.
